prove fill of extract

SSA/Projects/Tensor2D/Tensor2D.lean
@@ -10,6 +10,10 @@ structure Tensor2d' (α : Type) where
   n₁ : ℕ
   mat : Matrix (Fin n₀) (Fin n₁) α
 
+def Tensor2d'.error (α : Type) : Tensor2d' α where
+  n₀ := 0
+  n₁ := 0
+  mat := Matrix.of fun x _y => x.elim0
 
 def Tensor2d'.transpose (t : Tensor2d' α) : Tensor2d' α where
   n₀ := t.n₁
@@ -25,14 +29,16 @@ def Tensor2d'.map (f : α → β) (t : Tensor2d' α) : Tensor2d' β where
 
 theorem Tensor2d'.map_functorial (g : β → γ) (f : α → β) (t : Tensor2d' α) : t.map (g ∘ f) = (t.map f).map g := rfl
 
-
+theorem Tensor2d'.map_error (f : α → β) : (Tensor2d'.error α).map f = Tensor2d'.error β := by {
+  simp[map, error]
+}
 /-- K combinator / constant function. -/
 def const (a : α) (_b : β) : α := a
 
 def Tensor2d'.fill (v : β) (t : Tensor2d' α) : Tensor2d' β := t.map (const v)
 
 /-- extract a submatrix of (sz₀ × sz₁) size at offset (δ₀, δ₁). Fails if this is out of bounds. -/
-def Tensor2d'.extract (δ₀ δ₁ : ℕ) (sz₀ sz₁ : ℕ) (t : Tensor2d' α) : Option (Tensor2d' α) :=
+def Tensor2d'.extract (δ₀ δ₁ : ℕ) (sz₀ sz₁ : ℕ) (t : Tensor2d' α) : (Tensor2d' α) :=
   if SZ0 : δ₀ + sz₀ ≤ t.n₀ then
     if SZ1 : δ₁ + sz₁ ≤ t.n₁ then
       {
@@ -44,35 +50,37 @@ def Tensor2d'.extract (δ₀ δ₁ : ℕ) (sz₀ sz₁ : ℕ) (t : Tensor2d' α)
           t.mat ⟨δ₀ + ix₀, INBOUNDS0⟩ ⟨δ₁ + ix₁, INBOUNDS1⟩
         : Tensor2d' α
       }
-    else none
-  else none
+    else Tensor2d'.error (α := α)
+  else Tensor2d'.error (α := α)
 
 /-- This implies fill_extract -/
 theorem Tensor2d'.map_extract (δ₀ δ₁ sz₀ sz₁ : ℕ) (t : Tensor2d' α) (f : α → β) :
-  (t.map f).extract δ₀ δ₁ sz₀ sz₁ = (t.extract δ₀ δ₁ sz₀ sz₁).map (Tensor2d'.map f) := by {
+  (t.map f).extract δ₀ δ₁ sz₀ sz₁ = (t.extract δ₀ δ₁ sz₀ sz₁).map f := by {
     simp only [extract];
     have MAP_n₀ : (map f t).n₀ = t.n₀ := rfl
     simp only [MAP_n₀]
     have MAP_n₁ : (map f t).n₁ = t.n₁ := rfl
     simp only [MAP_n₁]
-    by_cases H₀ : δ₀ + sz₀ ≤ t.n₀ <;> simp[H₀];
-    by_cases H₁ : δ₁ + sz₁ ≤ t.n₁ <;> simp[H₁];
+    by_cases H₀ : δ₀ + sz₀ ≤ t.n₀ <;> simp[H₀, Tensor2d'.map_error];
+    by_cases H₁ : δ₁ + sz₁ ≤ t.n₁ <;> simp[H₁, Tensor2d'.map_error];
     simp only [map, Matrix.map, Matrix.of_apply, Int.ofNat_add_ofNat, Eq.ndrec, Int.rawCast, Int.cast_id,
       Nat.rawCast, Nat.cast_id, Int.ofNat_eq_coe, eq_mp_eq_cast, id_eq]
 }
 
 theorem Tensor2d'.fill_extract (δ₀ δ₁ sz₀ sz₁ : ℕ) (t : Tensor2d' α) (v : β) :
-  (t.fill v).extract δ₀ δ₁ sz₀ sz₁ = (t.extract δ₀ δ₁ sz₀ sz₁).map (Tensor2d'.fill v) := by {
+  (t.fill v).extract δ₀ δ₁ sz₀ sz₁ = (t.extract δ₀ δ₁ sz₀ sz₁).fill v := by {
     simp only[fill, Tensor2d'.map_extract]
 }
 
 
 inductive Op
 | add
-| const (v: Nat)
+-- TODO: generalize 'const'
+| constNat (v: Nat) | constTensor (t : Tensor2d' Int) | constInt (v : Int)
 | sub
 | map2d
 | fill2d
+| extract2d 
 
 inductive BaseType
 | int : BaseType
@@ -94,25 +102,33 @@ abbrev UserType := SSA.UserType BaseType
 def argUserType : Op → UserType
 | Op.add => ↑(BaseType.int, BaseType.int)
 | Op.sub => ↑(BaseType.int, BaseType.int)
-| Op.const _ => ()
+| Op.constNat _  => ()
+| Op.constTensor _  => ()
+| Op.constInt _  => ()
 | Op.map2d => BaseType.tensor2d
 | Op.fill2d => (BaseType.int, BaseType.tensor2d)
+| Op.extract2d => (((BaseType.nat, BaseType.nat), (BaseType.nat, BaseType.nat)), BaseType.tensor2d)
 
 @[simp]
 def outUserType : Op → UserType
 | Op.add => BaseType.int
 | Op.sub => BaseType.int
-| Op.const _ => BaseType.nat
+| Op.constNat _ => BaseType.nat 
+| Op.constTensor _ => BaseType.tensor2d
+| Op.constInt _ => BaseType.int
 | Op.map2d | Op.fill2d => BaseType.tensor2d
+| Op.extract2d => BaseType.tensor2d
 
 @[simp]
 def rgnDom : Op → UserType
-| Op.add | Op.sub | Op.const _ | Op.fill2d  => .unit
+| Op.add | Op.sub | Op.fill2d | Op.extract2d  => .unit
+| Op.constNat _ | Op.constTensor _ | Op.constInt _ => .unit
 | Op.map2d => BaseType.int
 
 @[simp]
 def rgnCod : Op → UserType
-| Op.add | Op.sub | Op.const _ | Op.fill2d  => .unit
+| Op.add | Op.sub | Op.fill2d  | Op.extract2d => .unit
+| Op.constNat _ | Op.constTensor _ | Op.constInt _ => .unit
 | Op.map2d => BaseType.int
 
 def eval (o : Op)
@@ -120,8 +136,10 @@ def eval (o : Op)
   (_rgn : (Goedel.toType (rgnDom o) → (Goedel.toType (rgnCod o)))) :
   (Goedel.toType (outUserType o)) :=
   match o with
-  | .const v => v
-  | .add =>
+  | .constNat v => v
+  | .constTensor v => v
+  | .constInt v => v
+  | .add => 
     let (x, y) := arg;
     let x : Int := x;
     let y : Int := y;
@@ -133,12 +151,15 @@ def eval (o : Op)
     x - y
   | .map2d => 
     let t : Tensor2d' Int := arg
-    let f : Int → Int := _rgn
+    let f : Int → Int := _rgn -- FAILS.
     t.map f
   | .fill2d => 
     let (v, t) : Int × Tensor2d' Int  := arg
     t.fill v
-
+  | .extract2d => 
+    let ((δ, sz), t) := arg
+    t.extract δ.fst δ.snd sz.fst sz.snd
+    
 instance TUS : SSA.TypedUserSemantics Op BaseType where
   argUserType := argUserType
   rgnDom := rgnDom
@@ -148,11 +169,19 @@ instance TUS : SSA.TypedUserSemantics Op BaseType where
 
 syntax "map2d" : dsl_op2
 syntax "fill2d" : dsl_op2
+syntax "extract2d" : dsl_op2
+syntax "constNat" "(" term ")" : dsl_op2
+syntax "constTensor" "(" term ")" : dsl_op2
+syntax "constInt" "(" term ")" : dsl_op2
 
 open EDSL2 in
 macro_rules
 | `([dsl_op2| map2d]) => `(Op.map2d)
 | `([dsl_op2| fill2d]) => `(Op.fill2d)
+| `([dsl_op2| extract2d]) => `(Op.extract2d)
+| `([dsl_op2| constNat($t)]) => `(Op.constNat $t)
+| `([dsl_op2| constTensor($t)]) => `(Op.constTensor $t)
+| `([dsl_op2| constInt($t)]) => `(Op.constInt $t)
 
 
 -- Why do these not get set?
@@ -165,31 +194,32 @@ register_simp_attr outUserType
 -- register_simp_attr BitVector.width
 register_simp_attr uncurry
 
--- TODO: what is the most convenient way to state extract?
--- TODO: there is no way in MLIR to talk about composition of functions, so `map . map` is out.
+-- NOTE: there is no way in MLIR to talk about composition of functions, so `map . map` is out
+--       as a peephole rewrite
 
+
+-- TODO: enable not writing the unit argument if not used.
+-- TOTHINK: See that there is no way to 
 open SSA EDSL2 in
-theorem map_fill_2d :
-  TSSA.eval (e := e) (Op := Op) (β := BaseType) [dsl_bb2|
-    return op:fill2d ($(i), op:map2d $(v), $(f))
+theorem map_fill_2d 
+    (t : Tensor2d' Int)
+    (sz₀ sz₁ ix₀ ix₁: Nat) 
+    (i : Int):
+  TSSA.eval
+  (e := e) (Op := Op) (β := BaseType) [dsl_bb2|
+    return op:fill2d (op:constInt(i) (), 
+      op:extract2d (
+          ((op:constNat(sz₀) () , op:constNat(sz₁) ()),
+           (op:constNat(ix₀) (), op:constNat(ix₁) ())),
+           op:constTensor(t) ()))
   ] =
   TSSA.eval (e := e) (Op := Op) (β := BaseType) [dsl_bb2|
-    return op:map2d (op:fill2d ($(i), $(v))), $(f)
+    return op:extract2d 
+      (((op:constNat(sz₀) (), op:constNat(sz₁) ()),
+        (op:constNat(ix₀) (), op:constNat(ix₁) ())),
+        op:fill2d (op:constInt(i) (), op:constTensor(t) ()))
   ] := by {
     dsimp only[TSSAIndex.eval, TSSA.eval]
-    -- TODO: at this point, why do we have (eval Op.map2d (TSSA.eval v fun T v => ...))? why is the TSSA.eval unfolded?
-    -- TODO: it seems to be that `(e arg)` in TSSA.eval gets evaluated eagerly. I do not want it to β-reduce this redex. Can I control this @chris?
-    -- TODO: at this point, having a tactic to find and replace subterms would be awesome.
-    -- TODO2: We should not let the proof state explode to this anyway.
-    simp[UserType.mkPair]
-    generalize I:(TSSA.eval i e) = ival 
-    generalize F:(TSSA.eval f EnvC.empty) = f 
-    generalize ARG:(TSSA.eval v fun T v =>
-          match T, v with
-          | T, Context.Var.prev v => e v
-          | .(UserType.UserType.ofBase BaseType.int), Context.Var.last => ival) = arg
-    -- TODO: this cannot even be generalized, even though it is the same subterm.
-    simp only[TypedUserSemantics.eval, eval]
-    rw[Tensor2d'.]
-    sorry
+    simp[UserType.mkPair, TypedUserSemantics.eval, eval]
+    simp[Tensor2d'.fill_extract]
   }
